examples/QueryStructure/WeatherwDelegation.v
@@ -1,5 +1,4 @@
-Require Import ADTSynthesis.QueryStructure.Automation.IndexSelection
-        ADTSynthesis.QueryStructure.Automation.AutoDB.
+Require Import ADTSynthesis.QueryStructure.Automation.AutoDB.
 
 Definition VALUE := "VALUE".
 Definition MEASUREMENT_TYPE := "MEASUREMENT_TYPE".
@@ -78,141 +77,18 @@ Definition WeatherSpec : ADT WeatherSig :=
               Return measurement!VALUE)
 }.
 
-Ltac CombineUse x y :=
-  fun a c =>
-    match goal with
-      | _ => x a c
-      | _ => y a c
-    end.
-
-Ltac foo :=
-  remove trivial insertion checks;
-    (* The trivial insertion checks involve the fresh id,
-       so we need to drill under the binder before
-       attempting to remove them. *)
-    rewrite refine_bind;
-    [ | reflexivity |
-      unfold pointwise_relation; intros; subst_strings;
-      repeat remove_trivial_insertion_constraints;
-      subst_strings;
-      (* These simplify and implement nontrivial constraint checks *)
-      repeat first
-             [ drop_symmetric_functional_dependencies
-             | fundepToQuery; try simplify with monad laws
-             | foreignToQuery; try simplify with monad laws
-             | setoid_rewrite refine_trivial_if_then_else; simplify with monad laws
-             ];
-             higher_order_reflexivity ];
-    finish honing.
-
-Ltac bar :=
-  simplify with monad laws;
-    subst_strings; repeat (setoid_rewrite DropQSConstraintsQuery_In; simpl);
-    repeat setoid_rewrite DropQSConstraintsQuery_In_UnderBinder;
-    simpl; pose_string_ids;
-    setoid_rewrite refineEquiv_pick_eq';
-    simplify with monad laws; cbv beta; simpl;
-    match goal with
-        H : DropQSConstraints_AbsR _ _ |- _ =>
-        unfold DropQSConstraints_AbsR in H; rewrite H
-    end;
-    finish honing.
-
-Definition WeatherSpec' : ADT WeatherSig.
-  let H := eval cbv delta [WeatherSpec
-                         QSGetNRelSchemaHeading GetNRelSchema
-                         GetNRelSchemaHeading Domain Specif.value
-                         IndexBound_tail IndexBound_head WeatherSpec] beta in WeatherSpec in
-      let H' := eval simpl in H in
-          exact H'.
-Defined.
-
-Definition SharpenedWeatherStation' :
-  sigT (fun adt => refineADT WeatherSpec' adt).
-Proof.
-  eexists.
-  Set Printing All.
-  Show Proof.
-  cbv beta delta [WeatherSpec' Specif.value].
-  pose_string_ids.
-  repeat match goal with
-               | |- context[BuildHeading ?attrlist] =>
-                 let heading := fresh "heading" in
-                 set (BuildHeading attrlist) as heading
-           end.
-  match goal with
-      |- context [@BuildADT (QueryStructure ?Rep) _ _ _ _] =>
-      eapply refineADT_BuildADT_Rep_refine_All with (AbsR := @DropQSConstraints_AbsR Rep);
-  [ repeat (first [eapply refine_Constructors_nil
-                        | eapply refine_Constructors_cons;
-                          [ intros;
-                            match goal with
-                              |  |- refine _ (?E _) => let H := fresh in set (H := E)
-                              | _ => idtac
-                            end | ] ])
-        | repeat (first [eapply refine_Methods_nil
-                        | eapply refine_Methods_cons;
-                          [ intros;
-                            match goal with
-                              |  |- refine _ (?E _ _) => let H := fresh in set (H := E)
-                              | _ => idtac
-                            end | ]
-                        ])]
-  end.
-  Show Proof.
-  apply Constructor_DropQSConstraints.
-  - subst heading; subst heading0; foo.
-  - foo.
-  - subst heading; subst heading0.
-    bar.
-  - subst heading; subst heading0; bar.
-Defined.
-
-
 Definition SharpenedWeatherStation :
   Sharpened WeatherSpec.
 Proof.
-  eapply SharpenStep.
-  eapply (projT2 SharpenedWeatherStation').
-  unfold SharpenedWeatherStation'; simpl.
   Start Profiling.
+  start honing QueryStructure.
 
   (* Old, explicit index selection*)
   (* make simple indexes using [[AREA_CODE]; [MEASUREMENT_TYPE; CELL_ID]]. *)
 
-  GenerateIndexesForAll
-    ClauseMatchers
-    ltac:(fun attrlist =>
-            match goal with
-              | [ |- Sharpened (@BuildADT (UnConstrQueryStructure ?sch) _ _ _ _ )] =>
-                let sch' := eval simpl in (qschemaSchemas sch) in
-                    makeIndex' sch' attrlist
-                               ltac:(fun l =>
-                                       let index := fresh "Index" in
-                                       pose l as index;
-                                     revert Index;
-                                     pose_string_ids;
-                                     repeat match goal with
-                                              | |- context [ ``(?R) ] =>
-                                                let idx := fresh in
-                                                set ``(R) as fresh in *
-                                              | |- context [@Build_BoundedIndex ?A ?Bound ?idx ?bnd] =>
-                                                let idx := fresh in
-                                                set (@Build_BoundedIndex A Bound idx bnd) as idx in *
-                                            end;
-                                     repeat match goal with
-                                              | |- context[BuildHeading ?attrlist] =>
-                                                let heading := fresh "heading" in
-                                                set (BuildHeading attrlist) as heading
-
-                                            end;
-                                     intros; cbv beta; simpl in *;
-                                       unfold Domain in *; simpl in *;
-                                       hone representation using (@DelegateToBag_AbsR sch index))
-            end).
+  make indexes using matchFindPrefixIndex.
   - initializer.
-  - subst heading; subst heading0.
-    insertion
+  - insertion
     ltac:(fun SC F indexed_attrs f k =>
             match goal with
               | _ => InclusionIndexUse SC F indexed_attrs f k
@@ -239,35 +115,7 @@ Proof.
                                           | _ => createLastInclusionTerm_dep dom f fds tail fs kind rest s k
                                           | _ => createLastRangeTerm_dep dom f fds tail fs kind rest s k
                                         end).
-  - subst heading; subst heading0.
-    insertion
-    ltac:(fun SC F indexed_attrs f k =>
-            match goal with
-              | _ => InclusionIndexUse SC F indexed_attrs f k
-              | _ => RangeIndexUse SC F indexed_attrs f k
-            end)
-           ltac:(fun f fds tail fs kind EarlyIndex LastIndex rest s k =>
-                   match goal with
-                     | _ => createEarlyInclusionTerm f fds tail fs kind EarlyIndex LastIndex rest s k
-                     | _ => createEarlyRangeTerm f fds tail fs kind EarlyIndex LastIndex rest s k
-                   end)
-                  ltac:(fun f fds tail fs kind s k =>
-                          match goal with
-                            | _ => createLastInclusionTerm f fds tail fs kind s k
-                            | _ => createLastRangeTerm f fds tail fs kind s k
-                          end)
-                         ltac:(fun SC F indexed_attrs visited_attrs f T k =>
-                                 match goal with
-                                   | _ => InclusionIndexUse_dep SC F indexed_attrs visited_attrs f T k
-                                   | _ => RangeIndexUse_dep SC F indexed_attrs visited_attrs f T k
-                                 end)
-                                randomCrab
-                                ltac:(fun dom f fds tail fs kind rest s k =>
-                                        match goal with
-                                          | _ => createLastInclusionTerm_dep dom f fds tail fs kind rest s k
-                                          | _ => createLastRangeTerm_dep dom f fds tail fs kind rest s k
-                                        end).
-  - observer
+  - insertion
     ltac:(fun SC F indexed_attrs f k =>
             match goal with
               | _ => InclusionIndexUse SC F indexed_attrs f k
@@ -321,131 +169,7 @@ Proof.
                                           | _ => createLastInclusionTerm_dep dom f fds tail fs kind rest s k
                                           | _ => createLastRangeTerm_dep dom f fds tail fs kind rest s k
                                         end).
-    Unset Printing All.
-    idtac.
-    simpl.
-    Set Printing All.
-    idtac.
-    Unset Printing All.
-    pose_string_ids.
-    repeat match goal with
-             | |- context [ ``(?R) ] =>
-               let idx := fresh in
-               set ``(R) as fresh in *
-             | |- context [@Build_BoundedIndex ?A ?Bound ?idx ?bnd] =>
-               let idx := fresh in
-               set (@Build_BoundedIndex A Bound idx bnd) as idx in *
-           end;
-      repeat match goal with
-               | |- context[BuildHeading ?attrlist] =>
-                 let heading := fresh "heading" in
-                 set (BuildHeading attrlist) as heading
-                                                  
-             end.
-    Set Printing All.
-    idtac.
-    repeat match goal with
-        |- context[IndexedQueryStructure ?qs_schema ?search_terms] =>
-        let repType := fresh "repType" in
-        set (IndexedQueryStructure qs_schema search_terms) as repType in *
-    end.
-    Check CallBagMethod.
-    repeat match goal with
-               |- appcontext[@CallBagMethod ?qs_schema (@icons ?A ?B ?a ?As ?b ?Bs)] => 
-               let index := fresh "Index" in
-               set (@icons A B a As b Bs) as index in *
-           end.
-    Print SearchUpdateTerms.
-    repeat match goal with
-               |- context [@Build_SearchUpdateTerms
-                             ?heading ?stType ?stMatcher
-                             ?utType ?utApply] =>
-               let stu := fresh "SearchUpdateTerm" in
-               set (@Build_SearchUpdateTerms heading stType stMatcher utType utApply) as stu in *
-           end.
-    Unset Printing All.
-    idtac.
-  - simpl.
-
-
-    subst_strings; pose_string_ids.
-  Set Printing All.
-  idtac.
-  honeOne
-    ltac:(fun SC F indexed_attrs f k =>
-            match goal with
-              | _ => InclusionIndexUse SC F indexed_attrs f k
-              | _ => RangeIndexUse SC F indexed_attrs f k
-            end)
-           ltac:(fun f fds tail fs kind EarlyIndex LastIndex rest s k =>
-                   match goal with
-                     | _ => createEarlyInclusionTerm f fds tail fs kind EarlyIndex LastIndex rest s k
-                     | _ => createEarlyRangeTerm f fds tail fs kind EarlyIndex LastIndex rest s k
-                   end)
-                  ltac:(fun f fds tail fs kind s k =>
-                          match goal with
-                            | _ => createLastInclusionTerm f fds tail fs kind s k
-                            | _ => createLastRangeTerm f fds tail fs kind s k
-                          end)
-                         ltac:(fun SC F indexed_attrs visited_attrs f T k =>
-                                 match goal with
-                                   | _ => InclusionIndexUse_dep SC F indexed_attrs visited_attrs f T k
-                                   | _ => RangeIndexUse_dep SC F indexed_attrs visited_attrs f T k
-                                 end)
-                                randomCrab
-                                ltac:(fun dom f fds tail fs kind rest s k =>
-                                        match goal with
-                                          | _ => createLastInclusionTerm_dep dom f fds tail fs kind rest s k
-                                          | _ => createLastRangeTerm_dep dom f fds tail fs kind rest s k
-                                        end).
-  Set Printing All.
-  idtac.
-  simpl.
-  subst_strings; pose_string_ids.
-  subst heading; subst heading0.
-  repeat match goal with
-           | |- context[BuildHeading ?attrlist] =>
-             let heading := fresh "heading" in
-             set (BuildHeading attrlist) as heading
-         end.
-  honeOne
-    ltac:(fun SC F indexed_attrs f k =>
-            match goal with
-              | _ => InclusionIndexUse SC F indexed_attrs f k
-              | _ => RangeIndexUse SC F indexed_attrs f k
-            end)
-           ltac:(fun f fds tail fs kind EarlyIndex LastIndex rest s k =>
-                   match goal with
-                     | _ => createEarlyInclusionTerm f fds tail fs kind EarlyIndex LastIndex rest s k
-                     | _ => createEarlyRangeTerm f fds tail fs kind EarlyIndex LastIndex rest s k
-                   end)
-                  ltac:(fun f fds tail fs kind s k =>
-                          match goal with
-                            | _ => createLastInclusionTerm f fds tail fs kind s k
-                            | _ => createLastRangeTerm f fds tail fs kind s k
-                          end)
-                         ltac:(fun SC F indexed_attrs visited_attrs f T k =>
-                                 match goal with
-                                   | _ => InclusionIndexUse_dep SC F indexed_attrs visited_attrs f T k
-                                   | _ => RangeIndexUse_dep SC F indexed_attrs visited_attrs f T k
-                                 end)
-                                randomCrab
-                                ltac:(fun dom f fds tail fs kind rest s k =>
-                                        match goal with
-                                          | _ => createLastInclusionTerm_dep dom f fds tail fs kind rest s k
-                                          | _ => createLastRangeTerm_dep dom f fds tail fs kind rest s k
-                                        end).
-  simpl.
-  subst_strings; pose_string_ids.
-  repeat match goal with
-           | |- context[BuildHeading ?attrlist] =>
-             let heading := fresh "heading" in
-             set (BuildHeading attrlist) as heading
-         end.
-  Print IndexedQueryStructure.
-
-        Set Printing All.
-        honeOne
+  - observer
     ltac:(fun SC F indexed_attrs f k =>
             match goal with
               | _ => InclusionIndexUse SC F indexed_attrs f k
@@ -473,15 +197,16 @@ Proof.
                                           | _ => createLastRangeTerm_dep dom f fds tail fs kind rest s k
                                         end).
 
-  Show Profile.
-  Time FullySharpenQueryStructure WeatherSchema Index.
-  simplify with monad laws.
-  Show Profile.
-  implement_bag_methods.
-  Show Profile.
-Time Defined.
+  - FullySharpenQueryStructure WeatherSchema Index;
+    implement_bag_methods.
+    Show Profile.
+    Time Defined. (* 83 seconds for Defined. *)
+
+(* This still takes forever. Maybe try w/o zeta?
 Time Definition WeatherStationImpl' : SharpenedUnderDelegates WeatherSig :=
-  Eval simpl in projT1 SharpenedWeatherStation. (* 28 --> 10 *)
+  Eval simpl in projT1 SharpenedWeatherStation. *)
+
+
 
 Print SharpenedWeatherStation.
 Print transitivity.
