src/QueryStructure/Automation/Constraints/ForeignKeyAutomation.v
@@ -12,15 +12,20 @@ Require Import Coq.Lists.List Coq.Arith.Compare_dec Coq.Bool.Bool Coq.Strings.St
         ADTSynthesis.Common.DecideableEnsembles
         ADTSynthesis.QueryStructure.Specification.Constraints.tupleAgree
         ADTSynthesis.QueryStructure.Specification.Operations.Mutate
-        ADTSynthesis.QueryStructure.Implementation.Constraints.ConstraintChecksRefinements.
+        ADTSynthesis.QueryStructure.Implementation.Constraints.ConstraintChecksRefinements
+        ADTSynthesis.QueryStructure.Automation.Common.
 
 Ltac foreignToQuery :=
-  match goal with
+      match goal with
     | [ |- context[{ b' | decides b' (ForeignKey_P ?AttrID ?AttrID' ?tupmap ?n (@GetUnConstrRelation ?qs_schema ?or ?TableID))}] ]
       =>
       let H' := fresh in
       pose (@refine_constraint_check_into_query
                         qs_schema TableID
                         (fun tup : Tuple => GetAttribute n AttrID = tupmap (GetAttribute tup AttrID')) or _) as H';
-        simpl in H'; setoid_rewrite H'; simplify with monad laws; cbv beta; simpl
+        unfold QSGetNRelSchemaHeading in H';
+        simpl in *;
+        pose_string_hyps; pose_heading_hyps;
+        fold_string_hyps_in H'; fold_heading_hyps_in H';
+        setoid_rewrite H'; simplify with monad laws; cbv beta; simpl; clear H'
   end.
