src/QueryStructure/Automation/SearchTerms/InclusionSearchTerms.v
@@ -1,0 +1,129 @@
+Require Import
+        Coq.Strings.String
+        ADTSynthesis.QueryStructure.Specification.Representation.QueryStructureNotations
+        ADTSynthesis.QueryStructure.Specification.SearchTerms.ListInclusion
+        ADTSynthesis.QueryStructure.Implementation.DataStructures.BagADT.IndexSearchTerms
+        ADTSynthesis.QueryStructure.Automation.IndexSelection.
+
+(* Instances for building indexes with make simple indexes. *)
+(* Every Kind of index is keyed on an inductive type with a single constructor*)
+Local Open Scope string_scope.
+Definition InclusionIndex : string := "InclusionIndex".
+
+(* This is our search term type. *)
+Record InvertedSearchTerm
+       (heading : Heading)
+  :=
+    { IndexSearchTerm : list string;
+      ItemSearchTerm : @Tuple heading -> bool }.
+
+(* This builds the type of searchterms and the matching function on them *)
+Global Instance InvertedIndexDenotation
+       (heading : Heading)
+       (index : @Attributes heading)
+       (projection : @Tuple heading -> list string)
+: @IndexDenotation "InclusionIndex" heading index :=
+  {| DenoteIndex := InvertedSearchTerm heading; (* Pick search term type *)
+     MatchIndex search_term item := (* matching function : DenoteIndex -> Tuple heading -> bool *)
+       if IncludedIn_dec (IndexSearchTerm search_term) (projection item) then
+         ItemSearchTerm search_term item
+       else false |}.
+
+(* Extra type class magic for inverted indices. *)
+Hint Extern 10 (@IndexDenotation "InclusionIndex" ?heading ?index) =>
+let index_domain := eval hnf in (@Domain heading index) in
+match index_domain with
+  | list string =>
+    apply (@InvertedIndexDenotation
+             heading index
+             (fun tup => GetAttribute tup index ))
+end
+: typeclass_instances.
+
+Ltac matchInclusionIndex WhereClause k :=
+  match WhereClause with
+    | fun tups => IncludedIn _ (@?C1 tups) =>
+      let attrs1 := TermAttributes C1 in
+      k (map (fun a12 => (InclusionIndex, (fst a12, snd a12)))
+             (attrs1))
+  end.
+
+Ltac InclusionIndexUse SC F indexed_attrs f k :=
+     match type of f with
+       (* Inclusion Search Terms *)
+       | forall a, {IncludedIn ?X (_!?fd)} + {_} =>
+          let H := fresh in
+          assert (List.In {| KindNameKind := "InclusionIndex";
+                             KindNameName := fd|} indexed_attrs) as H
+              by (clear; simpl; intuition eauto); clear H;
+            k ({| KindNameKind := "InclusionIndex";
+                  KindNameName := fd|}, X) (fun _ : @Tuple SC => true)
+        | forall a, {IncludedIn ?X (_``?fd)} + {_} =>
+          let H := fresh in
+          assert (List.In {| KindNameKind := "InclusionIndex";
+                             KindNameName := fd|} indexed_attrs) as H
+              by (clear; simpl; intuition eauto); clear H;
+            k ({| KindNameKind := "InclusionIndex";
+                  KindNameName := fd|}, X) (fun _ : @Tuple SC => true)
+     end.
+
+Ltac InclusionIndexUse_dep SC F indexed_attrs visited_attrs f T k :=
+  match type of f with
+    | forall a b, {IncludedIn (@?X a) (_!?fd)} + {_} =>
+          let H := fresh in
+          assert (List.In {| KindNameKind := "InclusionIndex";
+                             KindNameName := fd|} indexed_attrs) as H
+              by (clear; simpl; intuition eauto); clear H;
+          match eval simpl in
+                (in_dec string_dec fd visited_attrs) with
+            | right _ => k (fd :: visited_attrs)
+                           ({| KindNameKind := "InclusionIndex";
+                               KindNameName := fd |}, X)
+                           (fun (a : T) (_ : @Tuple SC) => true)
+            | left _ => k visited_attrs tt F
+          end
+        | forall a b, {IncludedIn (@?X a) (_``?fd)} + {_} =>
+          let H := fresh in
+          assert (List.In {| KindNameKind := "InclusionIndex";
+                             KindNameName := fd|} indexed_attrs) as H
+              by (clear; simpl; intuition eauto);
+            match eval simpl in
+                  (in_dec string_dec fd visited_attrs) with
+              | right _ => k (fd :: visited_attrs)
+                             ({| KindNameKind := "InclusionIndex";
+                                 KindNameName := fd |}, X)
+                             (fun (a : T) (_ : @Tuple SC) => true)
+              | left _ => k visited_attrs tt F
+            end
+  end.
+
+Ltac createLastInclusionTerm f fds tail fs kind s k :=
+  match kind with
+    | "InclusionIndex" =>
+      (findMatchingTerm
+         fds kind s
+         ltac:(fun X => k {| IndexSearchTerm := X;
+                             ItemSearchTerm := tail |}))
+        || k {| IndexSearchTerm := nil;
+                ItemSearchTerm := tail |}
+  end.
+
+Ltac createLastInclusionTerm_dep dom f fds tail fs kind rest s k :=
+  match kind with
+    | "InclusionIndex" =>
+      (findMatchingTerm
+         fds kind s
+         ltac:(fun X => k (fun x : dom => {| IndexSearchTerm := X x;
+                                             ItemSearchTerm := tail x |}))
+                || k (fun x : dom => {| IndexSearchTerm := nil;
+                                        ItemSearchTerm := tail x |}))
+  end.
+
+Ltac createEarlyInclusionTerm f fds tail fs kind EarlyIndex LastIndex rest s k :=
+  match kind with
+    | "InclusionIndex" =>
+      (findMatchingTerm
+         fds kind s
+         ltac:(fun X => k (X, rest)))
+        || k (@nil string, rest)
+  end.
